Machine integer handling in its own module

M6502_Reg.v
@@ -1,98 +1,8 @@
+Require Import MachineInt.
+
 (** This file defines the 6502 CPU registers. *)
 
-Require Import Coqlib.
-
-Module Type BitsM.
-
-  Parameter sz : nat.
-  Parameter szRange : sz = 8%nat \/ sz = 16%nat.
-
-End BitsM.
-
-Module FI(szM: BitsM).
-
-  Definition wordsize := szM.sz.
-
-  Definition sizeRange : wordsize = 8%nat \/ wordsize = 16%nat := szM.szRange.
-  Hint Resolve sizeRange : ints.
-
-  Definition modulus : Z := two_power_nat wordsize.
-  Definition half_modulus : Z := modulus / 2.
-
-Definition in_range (x: Z) :=
-  match x ?= 0 with
-  | Lt => False
-  | _  =>
-    match x ?= modulus with
-    | Lt => True
-    | _  => False
-    end
-  end.
-
-  Record int: Set := mkint { intval: Z; intrange: in_range intval }.
-
-Definition max_unsigned : Z := modulus - 1.
-Definition max_signed : Z := half_modulus - 1.
-Definition min_signed : Z := - half_modulus.
-
-Definition unsigned (n: int) : Z := intval n.
-
-Definition signed (n: int) : Z :=
-  if zlt (unsigned n) half_modulus
-  then unsigned n
-  else unsigned n - modulus.
-
-Lemma mod_in_range:
-  forall x, in_range (Zmod x modulus).
-Proof.
-  intro.
-  generalize (Z_mod_lt x modulus (two_power_nat_pos wordsize)).
-  intros [A B].
-  assert (C: x mod modulus >= 0). omega.
-  red. red in C. red in B. 
-  rewrite B. destruct (x mod modulus ?= 0); auto. 
-Qed.
-
-Definition repr (x: Z) : int := 
-  mkint (Zmod x modulus) (mod_in_range x).
-
-Definition zero := repr 0.
-Definition one  := repr 1.
-
-End FI.
-
-Module BYTE_SZ <: BitsM.
-
-  Definition sz := 8%nat.
-
-  Definition szRange : sz = 8%nat \/ sz = 16%nat.
-  Proof.
-    left.
-    unfold sz. auto.
-  Qed.
-
-End BYTE_SZ.
-
-Module WORD_SZ <: BitsM.
-
-  Definition sz := 16%nat.
-
-  Definition szRange : sz = 8%nat \/ sz = 16%nat.
-  Proof.
-    right.
-    unfold sz. auto.
-  Qed.
-
-End WORD_SZ.
-
-
-Module Byte := FI BYTE_SZ.
-Module Word := FI WORD_SZ.
-
-Definition byte := Byte.int.
-Definition word := Word.int.
-
-Inductive Reg8 : Set := A : Reg8 | X : Reg8 | Y : Reg8 | S : Reg8 | FLAGS : Reg8.
+Inductive Reg8 : Set := A : Reg8 | X : Reg8 | Y : Reg8 | STATUS : Reg8 | FLAGS : Reg8.
 Inductive Reg16 : Set := PC : Reg16.
 
 (** C : carry,
@@ -114,34 +24,45 @@ Inductive Flag : Set :=
   | FlagVF : Flag
   | FlagSF : Flag.
 
-Definition RegFile8 := Reg8 -> word.
+Definition RegFile8 := Reg8 -> byte.
 Definition RegFile16 := Reg16 -> word.
 
+(* Register State *)
 Definition RegFile := (list RegFile8 * RegFile16)%type.
 
-Definition setFlag (w: word) (f : Flag) : word :=
+Record RegF : Set :=
+  mkState {
+    RA: byte;
+    RX: byte;
+    RY: byte;
+    RSTATUS: byte;
+    RFLAGS: byte;
+    RPC: word
+  }.
+
+Definition setFlag (b: byte) (f: Flag): byte :=
   match f with
-  | FlagCF => Word.repr 1
-  | FlagZF => Word.repr 1
-  | FlagIF => Word.repr 1
-  | FlagDF => Word.repr 1
-  | FlagBF => Word.repr 1
-  | FlagVF => Word.repr 1
-  | FlagSF => Word.repr 1
+  | FlagCF => Byte.repr 1
+  | FlagZF => Byte.repr 1
+  | FlagIF => Byte.repr 1
+  | FlagDF => Byte.repr 1
+  | FlagBF => Byte.repr 1
+  | FlagVF => Byte.repr 1
+  | FlagSF => Byte.repr 1
   end.
 
-Definition clearFlag (w : word) (f : Flag) : word :=
+Definition clearFlag (b: byte) (f: Flag): byte :=
   match f with
-  | FlagCF => Word.repr 0
-  | FlagZF => Word.repr 0
-  | FlagIF => Word.repr 0
-  | FlagDF => Word.repr 0
-  | FlagBF => Word.repr 0
-  | FlagVF => Word.repr 0
-  | FlagSF => Word.repr 0
+  | FlagCF => Byte.repr 0
+  | FlagZF => Byte.repr 0
+  | FlagIF => Byte.repr 0
+  | FlagDF => Byte.repr 0
+  | FlagBF => Byte.repr 0
+  | FlagVF => Byte.repr 0
+  | FlagSF => Byte.repr 0
   end.
 
-Definition getFlag (w:word) (f : Flag) : bool :=
+Definition getFlag (b: byte) (f: Flag): bool :=
   match f with
   | FlagCF => false
   | FlagZF => false
@@ -151,4 +72,13 @@ Definition getFlag (w:word) (f : Flag) : bool :=
   | FlagVF => false
   | FlagSF => false
   end.
+
+(*Definition setReg8 : RegFile -> Reg8 -> byte -> RegFile :=
+  fun R r b =>
+    match r with
+      _ =>
+    end.
+
+Definition getReg8 : RegFile -> Reg8 -> byte :=
+  fun R r => _RF8 R r.*)
 
