MachineInt.v
@@ -1,0 +1,92 @@
+Require Import Coqlib.
+
+Module Type BitsM.
+
+  Parameter sz : nat.
+  Parameter szRange : sz = 8%nat \/ sz = 16%nat.
+
+End BitsM.
+
+Module FI(szM: BitsM).
+
+  Definition wordsize := szM.sz.
+
+  Definition sizeRange : wordsize = 8%nat \/ wordsize = 16%nat := szM.szRange.
+  Hint Resolve sizeRange : ints.
+
+  Definition modulus : Z := two_power_nat wordsize.
+  Definition half_modulus : Z := modulus / 2.
+
+Definition in_range (x: Z) :=
+  match x ?= 0 with
+  | Lt => False
+  | _  =>
+    match x ?= modulus with
+    | Lt => True
+    | _  => False
+    end
+  end.
+
+Record int: Set := mkint { intval: Z; intrange: in_range intval }.
+
+Definition max_unsigned : Z := modulus - 1.
+Definition max_signed : Z := half_modulus - 1.
+Definition min_signed : Z := - half_modulus.
+
+Definition unsigned (n: int) : Z := intval n.
+
+Definition signed (n: int) : Z :=
+  if zlt (unsigned n) half_modulus
+  then unsigned n
+  else unsigned n - modulus.
+
+Lemma mod_in_range:
+  forall x, in_range (Zmod x modulus).
+Proof.
+  intro.
+  generalize (Z_mod_lt x modulus (two_power_nat_pos wordsize)).
+  intros [A B].
+  assert (C: x mod modulus >= 0). omega.
+  red. red in C. red in B. 
+  rewrite B. destruct (x mod modulus ?= 0); auto. 
+Qed.
+
+Definition repr (x: Z) : int := 
+  mkint (Zmod x modulus) (mod_in_range x).
+
+Definition zero := repr 0.
+Definition one  := repr 1.
+
+End FI.
+
+Module BYTE_SZ <: BitsM.
+
+  Definition sz := 8%nat.
+
+  Definition szRange : sz = 8%nat \/ sz = 16%nat.
+  Proof.
+    left.
+    unfold sz. auto.
+  Qed.
+
+End BYTE_SZ.
+
+Module WORD_SZ <: BitsM.
+
+  Definition sz := 16%nat.
+
+  Definition szRange : sz = 8%nat \/ sz = 16%nat.
+  Proof.
+    right.
+    unfold sz. auto.
+  Qed.
+
+End WORD_SZ.
+
+
+Module Byte := FI BYTE_SZ.
+Module Word := FI WORD_SZ.
+
+Definition byte := Byte.int.
+Definition word := Word.int.
+
