refresh_makefile.sh
@@ -1,3 +1,0 @@
-#/bin/bash
-
-{ echo '-R . 6502Coq' ; find -name '*.v' -print; } > _CoqProject && coq_makefile -f _CoqProject -o Makefile
